Quicksort.fst
@@ -1,0 +1,114 @@
+module Quicksort
+
+// It's from the F* tutorial
+// http://www.fstar-lang.org/tutorial/
+
+open FStar.List
+
+let rec length l : nat =
+    match l with
+    | [] -> 0
+    | _ :: t -> 1 + length t
+
+let rec sorted (l:list int)
+  : bool
+  = match l with
+    | [] -> true
+    | [x] -> true
+    | x :: y :: xs -> x <= y && sorted (y :: xs)
+
+let rec mem (#a:eqtype) (i:a) (l:list a)
+  : bool
+  = match l with
+    | [] -> false
+    | hd :: tl -> hd = i || mem i tl
+
+let rec partition (#a:Type) (f:a -> bool) (l:list a)
+  : x:(list a & list a) { length (fst x) + length (snd x) = length l }
+  = match l with
+    | [] -> [], []
+    | hd::tl ->
+      let l1, l2 = partition f tl in
+      if f hd
+      then hd::l1, l2
+      else l1, hd::l2
+
+let rec sort (l:list int)
+  : Tot (list int) (decreases (length l))
+  = match l with
+    | [] -> []
+    | pivot :: tl ->
+      let hi, lo  = partition ((<=) pivot) tl in
+      append (sort lo) (pivot :: sort hi)
+
+let rec partition_mem (#a:eqtype)
+                      (f:(a -> bool))
+                      (l:list a)
+  : Lemma (let l1, l2 = partition f l in
+           (forall x. mem x l1 ==> f x) /\
+           (forall x. mem x l2 ==> not (f x)) /\
+           (forall x. mem x l = (mem x l1 || mem x l2)))
+  = match l with
+    | [] -> ()
+    | hd :: tl -> partition_mem f tl
+
+
+let rec sorted_concat (l1:list int{sorted l1})
+                      (l2:list int{sorted l2})
+                      (pivot:int)
+  : Lemma (requires (forall y. mem y l1 ==> not (pivot <= y)) /\
+                    (forall y. mem y l2 ==> pivot <= y))
+          (ensures sorted (append l1 (pivot :: l2)))
+  = match l1 with
+    | [] -> ()
+    | hd :: tl -> sorted_concat tl l2 pivot
+
+let rec append_mem (#t:eqtype)
+                   (l1 l2:list t)
+  : Lemma (ensures (forall a. mem a (append l1 l2) = (mem a l1 || mem a l2)))
+  = match l1 with
+    | [] -> ()
+    | hd::tl -> append_mem tl l2
+
+let rec sort_correct (l:list int)
+  : Lemma (ensures (
+           let m = sort l in
+           sorted m /\
+           (forall i. mem i l = mem i m)))
+          (decreases (length l))
+  = match l with
+    | [] -> ()
+    | pivot :: tl ->
+      let hi, lo  = partition ((<=) pivot) tl in
+      sort_correct hi;
+      sort_correct lo;
+      partition_mem ((<=) pivot) tl;
+      sorted_concat (sort lo) (sort hi) pivot;
+      append_mem (sort lo) (pivot :: sort hi)
+
+let sort_ok (l:list int) =
+    let m = sort l in
+    sorted m /\
+    (forall i. mem i l = mem i m)
+
+let rec sort_correct_annotated (l:list int)
+  : Lemma (ensures sort_ok l)
+          (decreases (length l))
+  = match l with
+    | [] -> ()
+    | pivot :: tl ->
+      let hi, lo  = partition ((<=) pivot) tl in
+      assert (length hi + length lo == length tl);
+      sort_correct_annotated hi;
+      assert (sort_ok hi);
+      sort_correct_annotated lo;
+      assert (sort_ok lo);
+      partition_mem ((<=) pivot) tl;
+      assert (forall i. mem i tl = mem i hi || mem i lo);
+      assert (forall i. mem i hi ==> pivot <= i);
+      assert (forall i. mem i lo ==> i < pivot);
+      assert (sort l == (append (sort lo) (pivot :: sort hi)));
+      sorted_concat (sort lo) (sort hi) pivot;
+      assert (sorted (sort l));
+      append_mem (sort lo) (pivot :: sort hi);
+      assert (forall i. mem i l = mem i (sort l))
